Almost finished the whole simulation proof. Axioms left for external calls.
One axiom says that the permissions of the stack blocks are unchanged. This is
to be put as an additional property of the external calls.
The other states that the unique stack block's permissions are unchanged by
external calls. This is subtler because there is no obvious way of
characterizing this stack block except from naming it explicitly.

x86/Asm.v
@@ -332,6 +332,13 @@ Definition set_pair (p: rpair preg) (v: val) (rs: regset) : regset :=
   | Twolong rhi rlo => rs#rhi <- (Val.hiword v) #rlo <- (Val.loword v)
   end.
 
+Fixpoint no_rsp_pair (b: rpair preg) :=
+  match b with
+    One r => r <> RSP
+  | Twolong hi lo => hi <> RSP /\ lo <> RSP
+  end.
+
+
 (** Assigning the result of a builtin *)
 
 Fixpoint set_res (res: builtin_res preg) (v: val) (rs: regset) : regset :=
@@ -339,6 +346,13 @@ Fixpoint set_res (res: builtin_res preg) (v: val) (rs: regset) : regset :=
   | BR r => rs#r <- v
   | BR_none => rs
   | BR_splitlong hi lo => set_res lo (Val.loword v) (set_res hi (Val.hiword v) rs)
+  end.
+
+Fixpoint no_rsp_builtin_preg (b: builtin_res preg) :=
+  match b with
+    BR r => r <> RSP
+  | BR_none => True
+  | BR_splitlong hi lo => no_rsp_builtin_preg lo /\ no_rsp_builtin_preg hi
   end.
 
 Section WITHEXTERNALCALLS.
@@ -1194,6 +1208,7 @@ Inductive step {exec_load exec_store} `{!MemAccessors exec_load exec_store} (ge:
       eval_builtin_args ge rs (rs RSP) m args vargs ->
       external_call ef ge vargs m t vres m' ->
       forall BUILTIN_ENABLED: builtin_enabled ef,
+        no_rsp_builtin_preg res ->
         rs' = nextinstr_nf
                 (set_res res vres
                          (undef_regs (map preg_of (destroyed_by_builtin ef)) rs)) ->
@@ -1216,6 +1231,7 @@ Inductive step {exec_load exec_store} `{!MemAccessors exec_load exec_store} (ge:
         (RA_NOT_VUNDEF: rs RA <> Vundef)
       ,      (* CompCertX: END additional conditions for calling convention *)
         external_call ef ge args m t res m' ->
+        no_rsp_pair (loc_external_result (ef_sig ef)) ->
         rs' = (set_pair (loc_external_result (ef_sig ef)) res (undef_regs (CR ZF :: CR CF :: CR PF :: CR SF :: CR OF :: nil) (undef_regs (map preg_of destroyed_at_call) rs))) #PC <- (rs RA) #RA <- Vundef ->
         step ge (State rs m) t (State rs' m').
 
@@ -1284,10 +1300,10 @@ Ltac Equalities :=
 + discriminate.
 + discriminate.
 + assert (vargs0 = vargs) by (eapply eval_builtin_args_determ; eauto). subst vargs0.
-  exploit external_call_determ. eexact H5. eexact H11. intros [A B].
+  exploit external_call_determ. eexact H5. eexact H12. intros [A B].
   split. auto. intros. destruct B; auto. subst. auto.
 + assert (args0 = args) by (eapply extcall_arguments_determ; eauto). subst args0.
-  exploit external_call_determ. eexact H4. eexact H9. intros [A B].
+  exploit external_call_determ. eexact H4. eexact H10. intros [A B].
   split. auto. intros. destruct B; auto. subst. auto.
 - (* trace length *)
   red; intros; inv H; simpl.
