x86/RawAsmgen.v
@@ -26,27 +26,21 @@ Section WITHMEMORYMODEL.
   
   Context `{memory_model: MemoryModelSingleStack}.
 
+  Inductive mono_initial_state {F V} (prog: program F V): state -> Prop :=
+  |mis_intro:
+     forall rs m m1 bstack,
+       initial_state prog (State rs m) ->
+       Mem.alloc m 0 (Memimpl.Mem.stack_limit) = (m1,bstack) ->
+       mono_initial_state prog (State rs m1).
+
   Existing Instance mem_accessors_default.
 
   Context `{!ExternalCallsOps mem} `{!EnableBuiltins mem}.
 
   Variable prog: Asm.program.
   Let ge := Genv.globalenv prog.
-
   Definition bstack: block := Genv.genv_next ge.
-  Variable id_stack: ident.
-
-  Variable tge: Genv.t Asm.fundef unit.
-  Hypothesis tge_plus_stack:
-    Genv.add_global ge (id_stack, Some (Gvar (mkglobvar tt nil false false))) = tge.
-
-  Lemma find_bstack: Genv.find_symbol tge id_stack = Some bstack.
-  Proof.
-    simpl; intros. subst.
-    unfold Genv.find_symbol. simpl.
-    rewrite Maps.PTree.gss.
-    reflexivity.
-  Qed.
+  Section PRESERVATION.
 
   Definition current_offset (v: val) :=
     match v with
@@ -203,9 +197,9 @@ Section WITHMEMORYMODEL.
         Mem.perm m b' o k p ->
         ~ ( delta + Z.max 0 (frame_size fi) <= o + delta' < delta + align (Z.max 0 (frame_size fi)) 8).
   
-  Inductive match_states: bool -> meminj -> Z -> state -> state -> Prop := 
+  Inductive match_states: meminj -> Z -> state -> state -> Prop :=
   | match_states_intro:
-      forall j b (rs: regset) m (rs': regset) m' 
+      forall j (rs: regset) m (rs': regset) m'
         (MINJ: Mem.inject j m m')
         (RSPzero: forall b o, rs # RSP = Vptr b o -> o = Ptrofs.zero )
         (RINJ: forall r, Val.inject j (rs # r) (rs' # r))
@@ -226,8 +220,14 @@ Section WITHMEMORYMODEL.
         (IS: inject_stack j (Mem.stack_adt m))
         (IP: inject_padding j m)
         (PS: perm_stack (Mem.stack_adt m) m)
-        (LRSP: b = true -> load_rsp (Mem.stack_adt m) m),
-        match_states b j (Ptrofs.unsigned ostack) (State rs m) (State rs' m').
+        (LRSP: load_rsp (Mem.stack_adt m) m)
+        (GLOBFUN_INJ: forall b f, Genv.find_funct_ptr ge b = Some f -> j b = Some (b,0))
+        (GLOBDEF_INJ: forall b f, Genv.find_def ge b = Some f -> j b = Some (b,0))
+        (GLOBSYMB_INJ: meminj_preserves_globals' ge j)
+        (GlobLe: (Genv.genv_next ge <= Mem.nextblock m)%positive)
+        (GlobLeT: (Genv.genv_next ge <= Mem.nextblock m')%positive)
+      ,
+        match_states j (Ptrofs.unsigned ostack) (State rs m) (State rs' m').
 
   Lemma inject_stack_incr:
     forall j j' (INCR: inject_incr j j')
@@ -268,339 +268,17 @@ Section WITHMEMORYMODEL.
     apply H. auto.
   Qed.
 
-  (* Lemma alloc_inject: *)
-  (*   forall j ostack m1 m2 (rs1 rs2: regset) fi m' b m1', *)
-  (*     match_states true j (Ptrofs.unsigned ostack) (State rs1 m1) (State rs2 m2) -> *)
-  (*     Mem.alloc m1 0 (frame_size fi) = (m', b) -> *)
-  (*     Mem.record_stack_blocks m' (Some (frame_with_info b (Some fi))) (frame_size fi) = Some m1' -> *)
-  (*     let curofs := current_offset (rs2 # RSP) in *)
-  (*     let newostack := offset_after_alloc curofs fi in *)
-  (*     let rs1' := (rs1 # RSP <- (Vptr b Ptrofs.zero)) in *)
-  (*     let rs2' := (rs2 # RSP <- (Vptr bstack (Ptrofs.repr newostack))) in *)
-  (*     exists j' m2', *)
-  (*       (forall bb, j' bb = if peq bb b then Some (bstack, newostack) else j bb)  *)
-  (*       /\ inject_incr j j' *)
-  (*       /\ Mem.record_stack_blocks m2 None (frame_size fi) = Some m2' *)
-  (*       /\ match_states false j' newostack (State rs1' m1') (State rs2' m2'). *)
-  (* Proof. *)
-  (*   intros j ostack m1 m2 rs1 rs2 fi m' b m1' MS ALLOC RSB curofs newostack rs1' rs2'. *)
-  (*   inv MS. *)
-  (*   assert (RSPDEC: (rs2 RSP = Vptr bstack ostack0 /\ curofs = Ptrofs.unsigned ostack0) *)
-  (*                   \/ (~ is_ptr (rs2 RSP) /\ curofs = Memimpl.Mem.stack_limit /\ Mem.stack_adt m1 = nil)). *)
-  (*   { *)
-  (*     destruct (is_ptr_dec (rs2 RSP)). *)
-  (*     left; destruct (rs2 RSP) eqn:?; simpl in *; try easy. *)
-  (*     specialize (RSPEQ _ _ eq_refl). *)
-  (*     intuition subst. auto. reflexivity. *)
-  (*     right. split; auto. *)
-  (*     split; auto. *)
-  (*     destruct (rs2 RSP) eqn:?; simpl in *; try easy. *)
-  (*     generalize (RINJ RSP). *)
-  (*     repeat destr_in AGSP1. *)
-  (*     rewrite H0. inversion 1. rewrite <- H4 in n. simpl in n; easy. *)
-  (*   } *)
-  (*   assert (REPRcur: align (Z.max 0 (frame_size fi)) 8 <= curofs <= Ptrofs.max_unsigned). *)
-  (*   { *)
-  (*     generalize (align_le (Z.max 0 (frame_size fi)) 8) (Z.le_max_l 0 (frame_size fi)). *)
-  (*     generalize (size_stack_below m1'). *)
-  (*     erewrite Mem.record_stack_blocks_stack_adt. 2: eauto. *)
-  (*     simpl. *)
-  (*     erewrite Mem.alloc_stack_blocks. 2: eauto. *)
-  (*     destruct (RSPDEC) as [[EQRSP ?]|[NOPTR [EQ NIL]]]; subst. *)
-  (*     unfold curofs, current_offset. rewrite EQRSP. erewrite AGSP; eauto. *)
-  (*     generalize (size_stack_pos (Mem.stack_adt m1)); intros. *)
-  (*     omega.  *)
-  (*     rewrite EQ, NIL. simpl. omega. *)
-  (*   } *)
-  (*   assert (REPR: 0 <= newostack <= Ptrofs.max_unsigned). *)
-  (*   { *)
-  (*     unfold newostack. *)
-  (*     unfold offset_after_alloc. *)
-  (*     generalize (align_le (Z.max 0 (frame_size fi)) 8) (Z.le_max_l 0 (frame_size fi)). *)
-  (*     omega. *)
-  (*   } *)
-  (*   generalize (Mem.alloc_left_mapped_inject _ _ _ _ _ _ _ _ newostack MINJ ALLOC VB). *)
-  (*   intro A. *)
-  (*   trim A. *)
-  (*   { *)
-  (*     omega. *)
-  (*   } *)
-  (*   trim A. *)
-  (*   { *)
-  (*     intros; right; eapply PBS; eauto. *)
-  (*   } *)
-  (*   trim A. *)
-  (*   { *)
-  (*     intros; eapply PBSL; eauto. *)
-  (*     split. omega. *)
-  (*     unfold newostack, offset_after_alloc. *)
-  (*     eapply Z.lt_le_trans with curofs. *)
-  (*     generalize (align_le (Z.max 0 (frame_size fi)) 8) (Z.le_max_l 0 (frame_size fi)). *)
-  (*     rewrite Z.max_r by omega. omega. *)
-  (*     destruct (RSPDEC) as [[EQRSP ?]|[NOPTR [EQ NIL]]]; subst.  *)
-  (*     rewrite H0. erewrite (AGSP _ EQRSP); eauto. *)
-  (*     generalize (size_stack_pos (Mem.stack_adt m1)); intros. omega. omega.  *)
-  (*   } *)
-  (*   trim A. *)
-  (*   { *)
-  (*     red. *)
-  (*     intros. *)
-  (*     unfold newostack, offset_after_alloc. *)
-  (*     eapply Zdivides_trans with 8. *)
-  (*     destruct chunk; try (exists 8; reflexivity); *)
-  (*       try (exists 4; reflexivity); *)
-  (*       try (exists 2; reflexivity); *)
-  (*       try (exists 1; reflexivity). *)
-  (*     apply Z.divide_sub_r. *)
-  (*     destruct (RSPDEC) as [[EQRSP ?]|[NOPTR [EQ NIL]]]; subst.  *)
-  (*     rewrite H0. apply SPAL; auto. *)
-  (*     rewrite EQ. auto. *)
-  (*     apply align_divides. omega. *)
-  (*   } *)
-  (*   trim A. *)
-  (*   { *)
-  (*     intros b0 delta' ofs k p JB PERM RNG. *)
-  (*     generalize (NIB _ _ _ _ _ JB PERM). *)
-  (*     destruct (RSPDEC) as [[EQRSP ?]|[NOPTR [EQ NIL]]]; subst.  *)
-  (*     rewrite EQRSP in RSPEQ. specialize (RSPEQ _ _ eq_refl). inv RSPEQ. *)
-  (*     generalize (align_le (frame_size fi) 8). *)
-  (*     unfold newostack, offset_after_alloc in RNG. *)
-  (*     rewrite Z.max_r in RNG by omega. simpl in RNG. omega. *)
-  (*     rewrite NIL in *. simpl. tauto.  *)
-  (*   } *)
-  (*   trim A. *)
-  (*   { *)
-  (*     revert NS. unfold no_stack. *)
-  (*     generalize (Mem.stack_adt m2). *)
-  (*     induction 1; simpl; intros; eauto. *)
-  (*     destruct x. simpl in *. rewrite H. *)
-  (*     simpl. intuition.  *)
-  (*   } *)
-  (*   destruct A as (f' & MINJ' & INCR & EQ1 & EQ2). *)
-  (*   exploit Mem.record_stack_blocks_inject. apply MINJ'. 4: eauto. *)
-  (*   instantiate (1:= None). simpl. auto. *)
-  (*   simpl. intros. split; auto. intro; subst. *)
-  (*   erewrite Mem.alloc_stack_blocks in H; eauto. *)
-  (*   eapply Mem.in_frames_valid in H. *)
-  (*   eapply Mem.fresh_block_alloc in H; eauto. *)
-  (*   red; easy. *)
-  (*   intros (m2' & RSB' & MINJ''). *)
-  (*   exists f', m2'. *)
-  (*   split; [|split;[|split]]. *)
-  (*   - intros. destruct peq; subst; auto. *)
-  (*   - red; intros. *)
-  (*     destruct (peq b0 b); auto. *)
-  (*   - eauto. *)
-  (*   - rewrite <- (Ptrofs.unsigned_repr newostack) by omega. *)
-  (*     econstructor; eauto. *)
-  (*     + intros b0 o A. unfold rs1' in A. rewrite Pregmap.gss in A. inv A; auto. *)
-  (*     + intros r. *)
-  (*       unfold rs1', rs2'. *)
-  (*       destruct (PregEq.eq r RSP). *)
-  (*       * subst. rewrite ! Pregmap.gss. *)
-  (*         econstructor; eauto. rewrite Ptrofs.add_zero_l; auto. *)
-  (*       * rewrite ! Pregmap.gso by auto. *)
-  (*         eapply val_inject_incr; eauto. *)
-  (*     + eapply Mem.record_stack_block_valid; eauto. *)
-  (*     + red. unfold rs2'. rewrite Pregmap.gss. inversion 1. subst. *)
-  (*       erewrite Mem.record_stack_blocks_stack_adt. 2: eauto. *)
-  (*       simpl. erewrite Mem.alloc_stack_blocks. 2: eauto. *)
-  (*       rewrite Ptrofs.unsigned_repr by auto. *)
-  (*       unfold newostack, offset_after_alloc in *. *)
-  (*       destruct (RSPDEC) as [[EQRSP ?]|[NOPTR [EQ NIL]]]; subst.  *)
-  (*       rewrite EQRSP in RSPEQ. specialize (RSPEQ _ _ eq_refl). inv RSPEQ. *)
-  (*       rewrite H0. rewrite (AGSP _ EQRSP). *)
-  (*       omega. *)
-  (*       rewrite EQ, NIL in *. simpl. omega. *)
-  (*     + erewrite Mem.record_stack_blocks_stack_adt. 2: eauto. simpl. *)
-  (*       unfold rs1'. apply Pregmap.gss. *)
-  (*     + red. intros ostack1 A. unfold rs2' in A; rewrite Pregmap.gss in A. *)
-  (*       inversion A. subst. *)
-  (*       rewrite Ptrofs.unsigned_repr by omega. *)
-  (*       unfold newostack. *)
-  (*       apply Z.divide_sub_r. *)
-  (*       destruct (RSPDEC) as [[EQRSP ?]|[NOPTR [EQ NIL]]]; subst.  *)
-  (*       rewrite H; apply SPAL; auto. *)
-  (*       rewrite EQ. auto. *)
-  (*       apply align_divides. omega. *)
-  (*     + red. intros ofs k p PERM. eapply Mem.record_stack_block_perm in PERM; eauto. *)
-  (*     + red; intros. eapply Mem.record_stack_block_perm'; eauto. *)
-  (*     + red; intros. erewrite Mem.record_stack_blocks_stack_adt. 2: eauto. constructor; auto. *)
-  (*     + unfold rs2'. rewrite Pregmap.gss. inversion 1. eauto. *)
-  (*     + rewrite Ptrofs.unsigned_repr by omega. *)
-  (*       red. intros b0 delta o k p JB PERM. *)
-  (*       eapply Mem.record_stack_block_perm in PERM. *)
-  (*       eapply Mem.perm_alloc_inv in PERM; eauto. *)
-  (*       2: eauto. *)
-  (*       destruct peq. *)
-  (*       * subst. rewrite EQ1 in JB. inv JB. split. omega. *)
-  (*         erewrite Mem.record_stack_blocks_stack_adt. 2: eauto. constructor; auto. *)
-  (*         simpl. auto. *)
-  (*       * split. unfold newostack, offset_after_alloc. *)
-  (*         transitivity curofs. *)
-  (*         -- generalize (Z.le_max_l 0 (frame_size fi)); intro MAX. *)
-  (*            generalize (align_le (Z.max 0 (frame_size fi)) 8). omega. *)
-  (*         --  *)
-  (*            destruct (RSPDEC) as [[EQRSP ?]|[NOPTR [EQ NIL]]]; subst.  *)
-  (*            rewrite H.  *)
-  (*            rewrite EQ2 in JB; auto.  *)
-  (*            exploit NIB; eauto. tauto. *)
-  (*            exploit NIB; eauto. rewrite <- EQ2. eauto. auto.  *)
-  (*            rewrite NIL. simpl; tauto. *)
-  (*         -- erewrite Mem.record_stack_blocks_stack_adt; eauto. *)
-  (*            erewrite Mem.alloc_stack_blocks; eauto. *)
-  (*            simpl. right. *)
-  (*            eapply NIB; eauto. rewrite <- EQ2; eauto. *)
-  (*     + erewrite Mem.record_stack_blocks_stack_adt; eauto. *)
-  (*       erewrite Mem.alloc_stack_blocks; eauto. *)
-  (*       constructor; auto. *)
-  (*       eapply inject_stack_incr; eauto. *)
-  (*       rewrite EQ1. f_equal. f_equal. *)
-  (*       unfold newostack, offset_after_alloc. *)
-  (*       destruct (RSPDEC) as [[EQRSP ?]|[NOPTR [EQ NIL]]]; subst. *)
-  (*       rewrite H. *)
-  (*       rewrite AGSP. omega. auto. rewrite EQ, NIL. simpl; omega. *)
-  (*     + intros b0 fi0 delta GFI FB0 b' o delta' k p FB1 P1. *)
-  (*       unfold Mem.get_frame_info in GFI. *)
-  (*       erewrite Mem.record_stack_blocks_stack_adt in GFI; eauto. *)
-  (*       erewrite Mem.alloc_stack_blocks in GFI; eauto. *)
-  (*       simpl in GFI. *)
-  (*       eapply Mem.record_stack_block_perm in P1. 2: eauto. *)
-  (*       eapply Mem.perm_alloc_inv in P1. 2: eauto.          *)
-  (*       destr_in GFI. *)
-  (*       * inv GFI. rewrite FB0 in EQ1; inv EQ1. *)
-  (*         destr_in P1. *)
-  (*         -- subst. rewrite FB0 in FB1; inv FB1. *)
-  (*            rewrite Z.max_r by omega.  omega. *)
-  (*         -- rewrite EQ2 in FB1 by auto. *)
-  (*            eapply NIB in P1; eauto. *)
-  (*            destruct P1 as (LE & IN). *)
-  (*            unfold newostack, offset_after_alloc. *)
-  (*            destruct (RSPDEC) as [[EQRSP EQA]|[NOPTR [EQA NIL]]]; subst; rewrite EQA. *)
-  (*            omega. rewrite NIL in IN; easy. *)
-  (*       *  *)
-  (*         rewrite EQ2 in FB0 by auto. *)
-
-  (*         Lemma perm_stack_eq: *)
-  (*           forall l m b fi, *)
-  (*             perm_stack l m -> *)
-  (*             get_assoc l b = Some fi -> *)
-  (*             forall o k p, *)
-  (*               Mem.perm m b o k p <-> 0 <= o < frame_size fi. *)
-  (*         Proof. *)
-  (*           induction 1; simpl; intros; eauto. congruence. *)
-  (*           destr_in H1. inv H1. *)
-  (*           auto. eauto. *)
-  (*         Qed. *)
-
-  (*         intro RNG. *)
-  (*         assert (0 < frame_size fi0). *)
-  (*         destruct (zlt 0 (frame_size fi0)); auto. *)
-  (*         rewrite Z.max_l in RNG by omega. change (align 0 8) with 0 in RNG. omega. *)
-  (*         rewrite Z.max_r in RNG by omega. *)
-
-  (*         destruct (RSPDEC) as [[EQRSP EQA]|[NOPTR [EQA NIL]]]; subst; rewrite EQA, ?NIL in *; try easy. *)
-          
-  (*         generalize (perm_stack_eq _ _ _ _ PS GFI). intro PF0.  *)
-
-  (*         destr_in P1. *)
-  (*         -- *)
-  (*           subst. rewrite EQ1 in FB1; inv FB1. *)
-
-  (*           cut (newostack + (frame_size fi)  <= delta). omega. *)
-  (*           unfold newostack. rewrite EQA. *)
-  (*           rewrite AGSP; auto. *)
-
-  (*           Lemma in_stack_inj_below: *)
-  (*             forall j l, *)
-  (*               inject_stack j l -> *)
-  (*               forall b fi, *)
-  (*             get_assoc l b = Some fi -> *)
-  (*             exists l1 l2, *)
-  (*               l = l1 ++ l2 /\ *)
-  (*               j b = Some (bstack, Memimpl.Mem.stack_limit - Memimpl.Mem.size_stack l2). *)
-  (*           Proof. *)
-  (*             induction 1; simpl; intros; eauto. *)
-  (*             congruence. *)
-  (*             destr_in H1; eauto. *)
-  (*             - subst. *)
-  (*               inv H1. *)
-  (*               rewrite H0. *)
-  (*               exists nil.  *)
-  (*               repeat eexists. *)
-  (*               f_equal. f_equal. simpl. omega.  *)
-  (*             - specialize (IHinject_stack _ _ H1). *)
-  (*               destruct IHinject_stack as (l1 & l2 & EQl & JB). *)
-  (*               subst. *)
-  (*               rewrite JB. *)
-  (*               repeat eexists. *)
-  (*               rewrite app_comm_cons. eauto. *)
-  (*           Qed. *)
-
-  (*           eapply in_stack_inj_below in GFI; eauto. *)
-  (*           destruct GFI as (l1 & l2 & EQADT & JB0). rewrite FB0 in JB0. inv JB0. *)
-  (*           rewrite Z.max_r in * by omega. *)
-
-  (*           unfold offset_after_alloc. *)
-  (*           rewrite Z.max_r by omega. *)
-
-  (*           cut (Memimpl.Mem.size_stack (Mem.stack_adt m1)  *)
-  (*                >= Memimpl.Mem.size_stack l2). *)
-  (*           generalize (align_le (frame_size fi) 8). omega. *)
-  (*           rewrite EQADT. *)
-
-  (*           Lemma size_stack_app: *)
-  (*             forall {A} (l1 l2: list (A * Z)), *)
-  (*               Memimpl.Mem.size_stack (l1 ++ l2) = Memimpl.Mem.size_stack l1 + Memimpl.Mem.size_stack l2. *)
-  (*           Proof. *)
-  (*             induction l1; simpl; intros; eauto. *)
-  (*             destruct a. *)
-  (*             rewrite IHl1. omega. *)
-  (*           Qed. *)
-  (*           rewrite size_stack_app. *)
-  (*           generalize (size_stack_pos l1); omega. *)
-
-  (*         -- eapply IP.  apply GFI. eauto. *)
-  (*            rewrite <- EQ2. apply FB1. auto. eauto. *)
-  (*            rewrite Z.max_r by omega. omega. *)
-                       
-             
-  (*     + erewrite Mem.record_stack_blocks_stack_adt; eauto. *)
-  (*       erewrite Mem.alloc_stack_blocks; eauto. *)
-  (*       constructor; auto. *)
-  (*       eapply perm_stack_inv. eauto. apply Mem.in_frames_valid. *)
-  (*       split; intros. *)
-  (*       eapply Mem.record_stack_block_perm in H0. 2: eauto. *)
-  (*       eapply Mem.perm_alloc_inv in H0; eauto. *)
-  (*       destr_in H0. *)
-  (*       subst. *)
-  (*       eapply Mem.in_frames_valid in H. *)
-  (*       eapply Mem.fresh_block_alloc in H. easy. *)
-  (*       eauto. *)
-  (*       eapply Mem.record_stack_block_perm'. eauto. *)
-  (*       eapply Mem.perm_alloc_1 in H0; eauto. *)
-  (*       split; intros. eapply Mem.record_stack_block_perm in H. 2: eauto. *)
-  (*       eapply Mem.perm_alloc_inv in H; eauto. *)
-  (*       rewrite pred_dec_true in H; auto. *)
-  (*       eapply Mem.record_stack_block_perm'. eauto. *)
-  (*       eapply Mem.perm_implies. *)
-  (*       eapply Mem.perm_alloc_2. eauto. auto. constructor. *)
-  (*     + congruence.         *)
-  (* Qed.        *)
-
-
   Axiom exec_instr_inject:
     forall j m1 m2 rs1 rs2 f i rs1' m1'
       (MINJ: Mem.inject j m1 m2)
       (RINJ: forall r, Val.inject j (rs1 # r) (rs2 # r))
       (IU: is_unchanged i = true)
       (EXEC: Asm.exec_instr ge f i rs1 m1 = Next rs1' m1'),
-      exists j' rs2' m2',
-        Asm.exec_instr tge f i rs2 m2 = Next rs2' m2'
-        /\ Mem.inject j' m1' m2'
-        /\ (forall r, Val.inject j' (rs1' # r) (rs2' # r))
-        /\ inject_incr j j'
-        /\ (forall b b' delta, j b = None -> j' b = Some (b', delta) -> Ple (Genv.genv_next ge) b /\ b' <> bstack). 
+      exists rs2' m2',
+        Asm.exec_instr ge f i rs2 m2 = Next rs2' m2'
+        /\ Mem.inject j m1' m2'
+        /\ (forall r, Val.inject j (rs1' # r) (rs2' # r))
+        (* /\ (forall b b' delta, j b = None -> j' b = Some (b', delta) -> Ple (Genv.genv_next ge) b /\ b' <> bstack) *). 
   (* should be proved already somewhere *)
 
   Lemma free_inject:
@@ -617,7 +295,6 @@ Section WITHMEMORYMODEL.
     auto. eapply Mem.free_left_inject. eauto. eauto. eauto.
     eauto.
   Qed.
-  
 
   Hypothesis type_init_sp:
     Val.has_type init_sp Tptr.
@@ -635,9 +312,6 @@ Section WITHMEMORYMODEL.
     intros; destruct (zle a b), (zle c d); try congruence; try omega.
     simpl in H; congruence.
   Qed.
-
-  
-
 
   Definition link_offsets l b o :=
     match get_assoc l b with
@@ -959,10 +633,49 @@ Section WITHMEMORYMODEL.
     apply val_inject_set; auto. 
     apply Val.offset_ptr_inject; auto.
   Qed.
-  
+
+  Lemma find_var_info_none_ge:
+    forall b,
+      (Genv.genv_next ge <= b)%positive ->
+      Genv.find_var_info ge b = None.
+  Proof.
+    unfold Genv.find_var_info. intros.
+    destr.
+    apply Genv.genv_defs_range in Heqo. xomega.
+  Qed.
+
+  Lemma load_record_stack_blocks:
+    forall m fi n m',
+      Mem.record_stack_blocks m fi n = Some m' ->
+      forall chunk b ofs,
+        Mem.load chunk m' b ofs = Mem.load chunk m b ofs.
+  Proof.
+    intros.
+    destruct (plt b (Mem.nextblock m)).
+    eapply Mem.load_unchanged_on_1.
+    eapply Mem.strong_unchanged_on_weak.
+    eapply Mem.record_stack_block_unchanged_on; eauto.
+    apply p.
+    instantiate (1 := fun _ _ => True); simpl; auto.
+    destruct (Mem.load chunk m b ofs) eqn:LOAD.
+    apply Mem.load_valid_access in LOAD. destruct LOAD.
+    exfalso; apply n0.
+    eapply Mem.perm_valid_block. apply H0.
+    instantiate (1:= ofs). generalize (size_chunk_pos chunk); omega.
+    clear LOAD.
+    destruct (Mem.load chunk m' b ofs) eqn:LOAD; auto.
+    apply Mem.load_valid_access in LOAD. destruct LOAD.
+    exfalso; apply n0.
+    eapply Mem.perm_valid_block.
+    specialize (H0 ofs). trim H0. generalize (size_chunk_pos chunk); omega.
+    rewrite_perms_bw H0.
+    apply H0.
+  Qed.
+
+
   Lemma alloc_inject:
     forall j ostack m1 (rs1 rs1': regset) fi b m1' m2 m3 m4 m5,
-      match_states true j (Ptrofs.unsigned ostack) (State rs1 m1) (State rs1' m1') ->
+      match_states j (Ptrofs.unsigned ostack) (State rs1 m1) (State rs1' m1') ->
       Mem.alloc m1 0 (frame_size fi) = (m2, b) ->
       Mem.store Mptr m2 b (seg_ofs (frame_link fi)) rs1#RSP = Some m3 ->
       Mem.store Mptr m3 b (seg_ofs (frame_retaddr fi)) rs1#RA = Some m4 ->
@@ -982,7 +695,7 @@ Section WITHMEMORYMODEL.
             exists m4',
               Mem.storev Mptr m3' (Val.offset_ptr (Vptr bstack (Ptrofs.repr newostack)) (Ptrofs.repr (seg_ofs (frame_retaddr fi)))) rs1'#RA = Some m4'
               /\ exists m5', Mem.record_stack_blocks m4' None (frame_size fi) = Some m5'
-                       /\ match_states true j' newostack (State rs2 m5) (State rs2' m5').
+                       /\ match_states j' newostack (State rs2 m5) (State rs2' m5').
   Proof.
     intros j ostack m1 rs1 rs1' fi b m1' m2 m3 m4 m5 MS ALLOC STORE_PARENT STORE_RETADDR RSB REPRlink REPRretaddr curofs newostack rs2 rs2'.
     inv MS.
@@ -1081,7 +794,7 @@ Section WITHMEMORYMODEL.
       destruct peq; subst; eauto.
     }
     split; auto.
-
+    (* store parent *)
     exploit Mem.store_mapped_inject. apply MINJ'. simpl in *; eauto. eauto.
     eapply val_inject_incr; eauto. intros (m3' & STORE & MINJ2).
     simpl.
@@ -1093,10 +806,9 @@ Section WITHMEMORYMODEL.
     intro VA; eapply Mem.store_valid_access_1 in VA; eauto. destruct VA.
     eapply H. rewrite Ptrofs.unsigned_repr; generalize (size_chunk_pos Mptr); omega.
     eexists; split; eauto.
-
+    (* store return address *)
     exploit Mem.store_mapped_inject. apply MINJ2. simpl in *; eauto. eauto. 
     eapply val_inject_incr; eauto. intros (m4' & STORE' & MINJ3).
-
     assert (Ptrofs.unsigned (Ptrofs.add (Ptrofs.repr newostack) (Ptrofs.repr (seg_ofs (frame_retaddr fi)))) =
             seg_ofs (frame_retaddr fi) + newostack) as EQ'.
     2: rewrite EQ', STORE'.
@@ -1108,7 +820,7 @@ Section WITHMEMORYMODEL.
     eapply H. 
     rewrite Ptrofs.unsigned_repr; generalize (size_chunk_pos Mptr); omega.
     eexists; split; eauto.
-
+    (* record the stack block *)
     exploit Mem.record_stack_blocks_inject. apply MINJ3. 4: eauto.
     instantiate (1:= None). simpl. auto.
     simpl. intros. split; auto. intro; subst.
@@ -1119,6 +831,7 @@ Section WITHMEMORYMODEL.
     intros (m5' & RSB' & MINJ'').
     rewrite RSB'.
     eexists; split; eauto.
+    (* proving the final match_states *)
     rewrite <- (Ptrofs.unsigned_repr newostack) by omega.
     econstructor; eauto.
     - intros b0 o A. unfold rs2 in A.
@@ -1250,7 +963,6 @@ Section WITHMEMORYMODEL.
       rewrite pred_dec_true in H; auto.
       do 3 rewrite_perms_fw. eapply Mem.perm_implies. eapply Mem.perm_alloc_2. eauto. eauto. constructor.
     - repeat rewrite_stack_blocks.
-      trim LRSP. auto. intros _.
       assert (Mem.unchanged_on (fun b o => in_frames (Mem.stack_adt m1) b) m1 m5).
       {
         eapply Mem.unchanged_on_trans.
@@ -1267,33 +979,8 @@ Section WITHMEMORYMODEL.
       eapply load_rsp_inv' in LRSP.
       eapply load_rsp_add. eauto.
 
-      Lemma load_record_stack_blocks:
-        forall m fi n m',
-          Mem.record_stack_blocks m fi n = Some m' ->
-          forall chunk b ofs,
-            Mem.load chunk m' b ofs = Mem.load chunk m b ofs.
-      Proof.
-        intros.
-        destruct (plt b (Mem.nextblock m)).
-        eapply Mem.load_unchanged_on_1.
-        eapply Mem.strong_unchanged_on_weak.
-        eapply Mem.record_stack_block_unchanged_on; eauto.
-        apply p.
-        instantiate (1 := fun _ _ => True); simpl; auto.
-        destruct (Mem.load chunk m b ofs) eqn:LOAD.
-        apply Mem.load_valid_access in LOAD. destruct LOAD.
-        exfalso; apply n0.
-        eapply Mem.perm_valid_block. apply H0.
-        instantiate (1:= ofs). generalize (size_chunk_pos chunk); omega.
-        clear LOAD.
-        destruct (Mem.load chunk m' b ofs) eqn:LOAD; auto.
-        apply Mem.load_valid_access in LOAD. destruct LOAD.
-        exfalso; apply n0.
-        eapply Mem.perm_valid_block.
-        specialize (H0 ofs). trim H0. generalize (size_chunk_pos chunk); omega.
-        rewrite_perms_bw H0.
-        apply H0.
-      Qed.
+
+
       erewrite load_record_stack_blocks. 2: eauto.
       erewrite Mem.load_store_other. 
       erewrite Mem.load_store_same. 
@@ -1335,7 +1022,35 @@ Section WITHMEMORYMODEL.
       destr_in H0.
       destruct (in_frames_dec (Mem.stack_adt m1) b0); auto.
       rewrite not_in_frames_get_assoc in Heqo; eauto; congruence.
-  Qed.       
+    - destruct GLOBSYMB_INJ; split.
+      + intros. eapply INCR. eauto.
+      + intros. destruct (peq b1 b).
+        subst; rewrite EQ1 in H2. inv H2.
+        simpl.
+        unfold Genv.block_is_volatile.
+        unfold Genv.find_var_info.
+        replace (Genv.find_def ge bstack) with (None (A:=globdef Asm.fundef unit)).
+        replace (Genv.find_def ge b) with (None (A:=globdef Asm.fundef unit)).
+        auto.
+        unfold Genv.find_def.
+        destruct (Maps.PTree.get b (Genv.genv_defs ge)) eqn:EQdef; auto.
+        apply Genv.genv_defs_range in EQdef.
+        exploit Mem.fresh_block_alloc. eauto. red. xomega. easy.
+        unfold Genv.find_def.
+        destruct (Maps.PTree.get bstack (Genv.genv_defs ge)) eqn:EQdef; auto.
+        apply Genv.genv_defs_range in EQdef.
+        unfold bstack in EQdef. xomega.
+        rewrite EQ2 in H2.
+        eauto.
+        auto.
+    - erewrite Mem.record_stack_block_nextblock. 2: eauto.
+      erewrite Mem.nextblock_store. 2 : eauto.
+      erewrite Mem.nextblock_store. 2 : eauto.
+      erewrite Mem.nextblock_alloc. 2: eauto. xomega.
+    - erewrite Mem.record_stack_block_nextblock. 2: eauto.
+      erewrite Mem.nextblock_store. 2 : eauto.
+      erewrite Mem.nextblock_store. 2 : eauto. xomega.
+  Qed.
 
   Lemma size_stack_divides {A} (l: list (A*Z)):
     (8 | Memimpl.Mem.size_stack l).
@@ -1396,20 +1111,20 @@ Section WITHMEMORYMODEL.
 
   Lemma exec_instr_inject':
     forall j ostack m1 m2 rs1 rs2 f i rs1' m1',
-      match_states true j ostack (State rs1 m1) (State rs2 m2) ->
+      match_states j ostack (State rs1 m1) (State rs2 m2) ->
       asm_instr_no_rsp i ->
       asm_instr_no_stack i ->
       Asm.exec_instr ge f i rs1 m1 = Next rs1' m1' ->
       exists j' ostack' rs2' m2',
-        exec_instr tge f i rs2 m2 = Next rs2' m2'
-        /\ match_states true j' ostack' (State rs1' m1') (State rs2' m2')
+        exec_instr ge f i rs2 m2 = Next rs2' m2'
+        /\ match_states j' ostack' (State rs1' m1') (State rs2' m2')
         /\ inject_incr j j'.
   Proof.
     intros j ostack m1 m2 rs1 rs2 f i rs1' m1' MS AINR AINS EI.
     destruct (is_unchanged i) eqn:?.
-    - edestruct exec_instr_inject as (j' & rs2' & m2' & EXEC' & MINJ' & RINJ' & INCR & NOSTACK); eauto.
+    - edestruct exec_instr_inject as (rs2' & m2' & EXEC' & MINJ' & RINJ'); eauto.
       inv MS; eauto. inv MS; eauto.
-      exists j', ostack, rs2', m2'; split; [|split]; eauto.
+      exists j, ostack, rs2', m2'; split; [|split]; eauto.
       destruct i; simpl in *; eauto; try congruence.
       inv MS; econstructor; eauto.
       + erewrite AINR; eauto.
@@ -1432,33 +1147,25 @@ Section WITHMEMORYMODEL.
       + erewrite AINR; eauto.
       + edestruct AINS. eauto. apply EI.
         red; intros.
-        rewrite H0 in H2.
-        destruct (j b) eqn:JB.
-        destruct p0.
-        rewrite H.
-        eapply NIB. rewrite JB. erewrite INCR in H1.
-        eauto.  eauto. eauto.
-        eapply NOSTACK in H1. 2: auto. 
-        intuition congruence.
+        edestruct AINS. eauto. apply EI. rewrite H3.
+        eapply NIB. auto. rewrite <- H4. eauto.
       + edestruct AINS. eauto. apply EI. rewrite H. eapply inject_stack_incr; eauto.
       + edestruct AINS. eauto. apply EI.
         red. unfold Mem.get_frame_info.
         rewrite H.
         intros b fi delta GFI JB b' o delta' k p JB' PERM RNG.
-        destruct (j b) eqn: JB0. destruct p0.
-        exploit INCR. rewrite JB0. eauto. rewrite JB. inversion 1; subst.
-        destruct (j b') eqn: JB'0. destruct p0.
-        exploit INCR. rewrite JB'0. eauto. rewrite JB'. inversion 1; subst.
         eapply IP. eauto. eauto. eauto. rewrite <- H0; eauto.
         apply RNG.
-        exploit NOSTACK. apply JB'0. apply JB'. intuition congruence.
-        exploit NOSTACK. apply JB0. apply JB. intuition congruence.
       + edestruct AINS. eauto. apply EI. rewrite H.
         eapply perm_stack_inv. eauto. apply Mem.in_frames_valid.
         intros; apply H0.
       + edestruct AINS. eauto. apply EI. rewrite H.
         intros; eapply load_rsp_inv'. eauto.
         eapply exec_instr_unchanged_on; eauto.
+      + etransitivity. apply GlobLe.
+        eapply asmgen_nextblock_forward; eauto.
+      + etransitivity. apply GlobLeT.
+        eapply asmgen_nextblock_forward; eauto.
 
     - destruct i; simpl in *; try congruence.
       + (* allocframe *)
@@ -1483,7 +1190,7 @@ Section WITHMEMORYMODEL.
         exists j',  newostack; eexists; eexists; split; eauto.
 
       + repeat destr_in EI.
-        inv MS. trim LRSP; auto.
+        inv MS.
         specialize (RSPzero _ _ Heqv1). subst.
         exploit Mem.loadv_inject. eauto. apply Heqo.
         apply Val.offset_ptr_inject. rewrite <- Heqv1; auto. intros (v2 & LOAD2 & INJ2).
@@ -1679,7 +1386,6 @@ Section WITHMEMORYMODEL.
           eapply inject_stack_norepeat in H0; eauto.
           simpl; auto.
         * inversion LRSP. constructor.
-          intro.
           rewrite <- H6 in *.
           eapply load_rsp_inv'. eauto.
           eapply Mem.unchanged_on_trans.
@@ -1689,7 +1395,7 @@ Section WITHMEMORYMODEL.
           simpl.
           intros. 
           intro; subst.
-          red in H11. destr_in H11. simpl in Heqo3. destr_in Heqo3. subst. xomega.
+          red in H10. destr_in H10. simpl in Heqo3. destr_in Heqo3. subst. xomega.
           exploit inject_stack_norepeat. apply LRSP. simpl. eauto.
           simpl.
           destruct (in_frames_dec l b); auto.
@@ -1697,57 +1403,789 @@ Section WITHMEMORYMODEL.
           eapply Mem.strong_unchanged_on_weak.
           eapply Mem.unrecord_stack_block_unchanged_on.
           eauto.
+        * etransitivity. apply GlobLe.
+          erewrite <- Mem.nextblock_free. 2: eauto.
+          erewrite <- Mem.unrecord_stack_block_nextblock.
+          2: eauto. xomega.
+       * etransitivity. apply GlobLeT.
+          erewrite <- Mem.unrecord_stack_block_nextblock.
+          2: eauto. xomega.
   Qed.
-  
-  Theorem step_simulation:
-    forall S1 t S2, Asm.step ge S1 t S2 ->
-               forall S1' (MS: match_states S1 S1'),
-                 (exists S2', step ge S1' t S2' /\ match_states S2 S2').
+
+  Definition asm_prog_no_rsp (ge: Genv.t Asm.fundef unit):=
+    forall b f,
+      Genv.find_funct_ptr ge b = Some (Internal f) ->
+      asm_code_no_rsp (fn_code f).
+
+  Hypothesis prog_no_rsp: asm_prog_no_rsp ge.
+
+  Existing Instance symbols_inject_instance.
+  Context `{ecprops: !ExternalCallsProps mem}.
+
+  Axiom external_call_perm_frames:
+    forall {F V} ef (ge: Genv.t F V) args m1 t res m2,
+      external_call ef ge args m1 t res m2 ->
+      forall b o k p,
+        in_frames (Mem.stack_adt m1) b ->
+        Mem.perm m2 b o k p <-> Mem.perm m1 b o k p.
+
+
+  Axiom external_call_perm_bstack:
+    forall {F V} ef (ge: Genv.t F V) args m1 t res m2,
+      external_call ef ge args m1 t res m2 ->
+      forall o k p,
+        Mem.perm m2 bstack o k p <-> Mem.perm m1 bstack o k p.
+
+
+  Lemma inj_incr_sep_same:
+    forall j j' m1 m2 b1 b2 delta,
+      inject_incr j j' ->
+      inject_separated j j' m1 m2 ->
+      j' b1 = Some (b2, delta) ->
+      Mem.valid_block m2 b2 ->
+      j b1 = Some (b2, delta).
   Proof.
-    destruct 1; intros; inv MS.
-    -
+    intros.
+    destruct (j b1) eqn:JB.
+    destruct p. eapply H in JB; eauto.
+    congruence.
+    exploit H0; eauto. intuition congruence.
+  Qed.
+
+  Lemma in_link_not_in_data:
+    forall f o,
+      in_segment o (frame_link f)
+      -> ~ in_stack_data o (o + 1) f.
+  Proof.
+    clear. intros f o IS ISD.
+    eapply frame_disjoints in IS.
+    apply IS. do 4 right; left.
+    apply ISD. omega.
+  Qed.
+
+  Lemma set_res_no_rsp:
+    forall res vres rs,
+      no_rsp_builtin_preg res ->
+      set_res res vres rs RSP = rs RSP.
+  Proof.
+    induction res; simpl.
+    - intros. eapply Pregmap.gso. auto.
+    - auto.
+    - intros vres rs (NR1 & NR2).
+      rewrite IHres2; auto.
+  Qed.
+
+  Lemma val_inject_set_res:
+    forall r rs1 rs2 v1 v2 j,
+      Val.inject j v1 v2 ->
+      (forall r0, Val.inject j (rs1 r0) (rs2 r0)) ->
+      forall r0, Val.inject j (set_res r v1 rs1 r0) (set_res r v2 rs2 r0).
+  Proof.
+    induction r; simpl; intros; auto.
+    apply val_inject_set; auto.
+    eapply IHr2; eauto.
+    apply Val.loword_inject. auto.
+    intros; eapply IHr1; eauto.
+    apply Val.hiword_inject. auto.
+  Qed.
+
+  Definition init_data_diff (id: init_data) (i: ident) :=
+    match id with
+      Init_addrof ii _ => ii <> i
+    | _ => True
+    end.
+
+  Lemma store_init_data_eq:
+    forall F V m (ge: _ F V) id gv b o i,
+      init_data_diff i id ->
+      Genv.store_init_data (Genv.add_global ge (id,gv)) m b o i =
+      Genv.store_init_data ge m b o i.
+  Proof.
+    destruct i; simpl; intros; auto.
+    unfold Genv.find_symbol; simpl. 
+    rewrite Maps.PTree.gso; auto.
+  Qed.
+
+  Lemma store_init_data_list_eq:
+    forall F V id i, 
+      Forall (fun x => init_data_diff x id) i ->
+      forall m (ge: _ F V) gv b o,
+        Genv.store_init_data_list (Genv.add_global ge (id,gv)) m b o i =
+        Genv.store_init_data_list ge m b o i.
+  Proof.
+    induction 1; simpl; intros; auto.
+    rewrite store_init_data_eq; auto.
+    destr. 
+  Qed.
+
+  Lemma alloc_global_eq:
+    forall F V (l: (ident * option (globdef F V))) m (ge: _ F V) id gv,
+      (forall v, snd l = Some (Gvar v) -> Forall (fun x => init_data_diff x id) (gvar_init v)) ->
+      Genv.alloc_global (Genv.add_global ge (id,gv)) m l =
+      Genv.alloc_global ge m l .
+  Proof.
+    destruct l; simpl; intros.
+    repeat (destr; [idtac]).
+    rewrite store_init_data_list_eq. auto.
+    apply H; auto.
+  Qed.
+
+  Lemma alloc_globals_eq:
+    forall F V (l: list (ident * option (globdef F V))) m (ge: _ F V) id gv,
+      (forall x v, In x l -> snd x = Some (Gvar v) -> Forall (fun x => init_data_diff x id) (gvar_init v)) ->
+      Genv.alloc_globals (Genv.add_global ge (id,gv)) m l =
+      Genv.alloc_globals ge m l .
+  Proof.
+    induction l; simpl; intros; eauto.
+    rewrite alloc_global_eq. destr.
+    apply IHl. intros; eauto.
+    eauto.
+  Qed.
+
+  Lemma find_symbol_add_globals_other:
+    forall F V l (ge: _ F V) s,
+      ~ In s (map fst l) ->
+      Genv.find_symbol (Genv.add_globals ge l) s =
+      Genv.find_symbol ge s.
+  Proof.
+    induction l; simpl; intros; eauto.
+    rewrite IHl.
+    unfold Genv.find_symbol; simpl.
+    apply Maps.PTree.gso. intuition. intuition.
+  Qed.
+
+
+  Lemma find_symbol_add_global_other:
+    forall F V l (ge: _ F V) s,
+      s <> fst l ->
+      Genv.find_symbol (Genv.add_global ge l) s =
+      Genv.find_symbol ge s.
+  Proof.
+    destruct l; simpl; intros; eauto.
+    unfold Genv.find_symbol; simpl.
+    apply Maps.PTree.gso. intuition. 
+  Qed.
+
+  Lemma find_symbol_none_add_global:
+    forall F V (ge: Genv.t F V) a i,
+      Genv.find_symbol (Genv.add_global ge a) i = None ->
+      i <> fst a /\ Genv.find_symbol ge i = None.
+  Proof.
+    unfold Genv.find_symbol; simpl.
+    intros F V ge0 a i.
+    rewrite Maps.PTree.gsspec.
+    destr.
+  Qed.
+
+  Lemma find_symbol_none_add_globals:
+    forall F V a (ge: Genv.t F V) i,
+      Genv.find_symbol (Genv.add_globals ge a) i = None ->
+      ~ In i (map fst a) /\ Genv.find_symbol ge i = None.
+  Proof.
+    induction a; simpl; intros; eauto.
+    apply IHa in H.
+    destruct H as (H1 & H).
+    apply find_symbol_none_add_global in H; auto.
+    intuition.
+  Qed.
+
+  Lemma find_symbol_none_not_in_defs:
+    forall F V (p: program F V) i,
+      Genv.find_symbol (Genv.globalenv p) i = None ->
+      ~ In i (map fst (prog_defs p)).
+  Proof.
+    unfold Genv.globalenv.
+    intros F V p.
+    generalize (Genv.empty_genv F V (prog_public p)).
+    generalize (prog_defs p).
+    induction l; simpl; intros; eauto.
+    apply find_symbol_none_add_globals in H.
+    destruct H as (A & B).
+    apply find_symbol_none_add_global in B.
+    destruct B as (B & C).
+    intuition.    
+  Qed.
+
+ 
+
+
+  Lemma extcall_arg_inject:
+    forall j rs1 m1 arg1 loc rs2 m2,
+      extcall_arg rs1 m1 loc arg1 ->
+      (forall r, Val.inject j (rs1 r) (rs2 r)) ->
+      Mem.inject j m1 m2 ->
+      exists arg2,
+        extcall_arg rs2 m2 loc arg2 /\
+        Val.inject j arg1 arg2.
+  Proof.
+    destruct 1; simpl; intros.
+    eexists; split; try econstructor; eauto.
+    exploit Mem.loadv_inject; eauto.
+    apply Val.offset_ptr_inject; eauto.
+    intros (v2 & LOAD & INJ).
+    eexists; split; try econstructor; eauto.
+  Qed.
+
+  Lemma extcall_arg_pair_inject:
+    forall j rs1 m1 arg1 ty rs2 m2,
+      extcall_arg_pair rs1 m1 ty arg1 ->
+      (forall r, Val.inject j (rs1 r) (rs2 r)) ->
+      Mem.inject j m1 m2 ->
+      exists arg2,
+        extcall_arg_pair rs2 m2 ty arg2 /\
+        Val.inject j arg1 arg2.
+  Proof.
+    destruct 1; simpl; intros.
+    eapply extcall_arg_inject in H; eauto.
+    destruct H as (arg2 & EA & INJ);
+      eexists; split; try econstructor; eauto.
+    eapply extcall_arg_inject in H; eauto.
+    destruct H as (arg2 & EA & INJ).
+    eapply extcall_arg_inject in H0; eauto.
+    destruct H0 as (arg3 & EA1 & INJ1).
+    eexists; split; try econstructor; eauto.
+    apply Val.longofwords_inject; eauto.
+  Qed.
+
+  Lemma extcall_arguments_inject:
+    forall j rs1 m1 args1 sg rs2 m2,
+      extcall_arguments rs1 m1 sg args1 ->
+      (forall r, Val.inject j (rs1 r) (rs2 r)) ->
+      Mem.inject j m1 m2 ->
+      exists args2,
+        extcall_arguments rs2 m2 sg args2 /\
+        Val.inject_list j args1 args2.
+  Proof.
+    unfold extcall_arguments.
+    intros j rs1 m1 args1 sg rs2 m2.
+    revert args1. generalize (loc_arguments sg).
+    induction 1; simpl; intros; eauto.
+    exists nil; split; try econstructor.
+    eapply extcall_arg_pair_inject in H; eauto.
+    decompose [ex and] H.
+    edestruct IHlist_forall2 as (a2 & EA & INJ); eauto.
+    eexists; split; econstructor; eauto.
+  Qed.
+
+  Theorem step_simulation:
+    forall S1 t S2,
+      Asm.step ge S1 t S2 ->
+      forall j ostack S1' (MS: match_states j ostack S1 S1'),
+      exists j' ostack' S2',
+        step ge S1' t S2' /\
+        match_states j' ostack' S2 S2'.
+  Proof.
+    destruct 1; intros; inversion MS; subst.
+    - 
       generalize (RINJ PC); rewrite H. inversion 1; subst.
       assert (j b = Some (b,0)) as JB.
       {
-        destruct MPG.
-        apply DOMAIN.
-        eapply FUNCTIONS. eauto. 
+        eapply GLOBFUN_INJ. eauto.
       }
       rewrite JB in H7; inv H7. 
-      generalize (exec_instr_inject _ _ _ _ _ _ _ _ _ MINJ RINJ H2).
-      intros (j' & rs2' & m2' & EI & MINJ' & RINJ' & INCR).
-      destruct (is_unchanged i) eqn:?.
-      eexists; split.
+      assert (asm_instr_no_rsp i).
+      {
+        eapply prog_no_rsp. eauto.
+        eapply Asmgenproof0.find_instr_in; eauto.
+      }
+      
+      destruct (exec_instr_inject' _ _ _ _ _ _ _ _ _ _ MS H4 (asmgen_no_change_stack i) H2)
+        as ( j' & ostack' & rs2' & m2' & EI' & MS' & INCR).
+      do 3 eexists; split.
       eapply exec_step_internal; eauto.
       rewrite Ptrofs.add_zero. eauto.
-      instantiate (1 := m2'). instantiate (1:= rs2').
-      rewrite <- EI. destruct i; simpl in *; try congruence.
-      econstructor; eauto.
-      admit.
-      destruct i; simpl in Heqb; try congruence.
-      + 
-        eexists; split.
-        eapply exec_step_internal; eauto.
-        rewrite Ptrofs.add_zero. eauto.
-        instantiate (1 := m2'). instantiate (1:= rs2').
-
-
-        simpl in EI.
-        eapply Ageneralize (Genv.find_funct_ptr_transf match_prog _ H0). intro FFP.
-      generalize (find_instr_transl _ _ _ H1); intro FINSTR.
-
-      assert (match i with
-                Pallocframe _ _ _
-              | Pfreeframe _ _ _ => False
-              | _ => True
-              end \/ (match i with
-                Pallocframe _ _ _
-              | Pfreeframe _ _ _ => True
-              | _ => False
-              end)) as DEC.
+      eauto.
+    -
+      edestruct (eval_builtin_args_inject) as (vargs' & Hargs & Hargsinj).
+      6: eauto.
+      eauto. eauto. eauto.
+      eauto. 
+      eapply GLOBSYMB_INJ.
+      edestruct (external_call_mem_inject_gen ef ge ge)
+        as (j' & vres' & m2' & EC & RESinj & MemInj & Unch1 & Unch2 & INCR & SEP).
+      apply meminj_preserves_globals'_symbols_inject.
+      eauto.
+      eauto.
+      eauto.
+      eauto. 
+      generalize (RINJ PC); rewrite H. inversion 1; subst.
+      assert (j b = Some (b,0)) as JB.
       {
-        destruct i; simpl; auto.
+        eapply GLOBFUN_INJ. eauto.
       }
-      destruct DEC.
+      rewrite JB in H9; inv H9. 
+      
+      do 3 eexists; split.
+      eapply exec_step_builtin.
+      eauto.
+      eauto. 
+      rewrite Ptrofs.add_zero; eauto.
+      eauto.
+      eauto.
+      auto.
+      reflexivity.
+      econstructor.
+      + eauto.
+      + rewrite nextinstr_nf_rsp.
+        intros b o.
+        rewrite set_res_no_rsp.
+        rewrite Asmgenproof0.undef_regs_other.
+        eauto.
+        intros; intro; subst. rewrite in_map_iff in H6.
+        destruct H6 as (x & EQ & IN).
+        apply preg_of_not_rsp in EQ. congruence.
+        auto.
+      + intros. apply val_inject_nextinstr_nf.
+        apply val_inject_set_res; auto.
+        apply val_inject_undef_regs; auto.
+        intros; eapply val_inject_incr; eauto.
+      + eapply external_call_valid_block; eauto.
+      + red. rewrite nextinstr_nf_rsp.
+        rewrite set_res_no_rsp; auto.
+        rewrite Asmgenproof0.undef_regs_other.
+        erewrite <- external_call_stack_blocks. eauto. eauto.
+        intros; intro; subst.
+        rewrite in_map_iff in H6.
+        destruct H6 as (x & EQ & IN).
+        apply preg_of_not_rsp in EQ. congruence.
+      + erewrite <- external_call_stack_blocks. 2: eauto.
+        rewrite nextinstr_nf_rsp.
+        rewrite set_res_no_rsp; auto.
+        rewrite Asmgenproof0.undef_regs_other. eauto.
+        intros; intro; subst.
+        rewrite in_map_iff in H6.
+        destruct H6 as (x & EQ & IN).
+        apply preg_of_not_rsp in EQ. congruence.
+      + red. 
+        rewrite nextinstr_nf_rsp.
+        rewrite set_res_no_rsp; auto.
+        rewrite Asmgenproof0.undef_regs_other. eauto.
+        intros; intro; subst.
+        rewrite in_map_iff in H6.
+        destruct H6 as (x & EQ & IN).
+        apply preg_of_not_rsp in EQ. congruence.
+      + red.
+        intros.
+        eapply Mem.perm_max in H6.
+        eapply external_call_max_perm in H6.
+        2: eauto.
+        eauto. eauto.
+      + red.
+        intros.
+        eapply external_call_perm_bstack. eauto.
+        eauto.
+      + red.
+        erewrite <- external_call_stack_blocks. 2: eauto.
+        eauto.
+      + rewrite nextinstr_nf_rsp.
+        rewrite set_res_no_rsp; auto.
+        rewrite Asmgenproof0.undef_regs_other. eauto.
+        intros; intro; subst.
+        rewrite in_map_iff in H6.
+        destruct H6 as (x & EQ & IN).
+        apply preg_of_not_rsp in EQ. congruence.
+      + red. intros b delta o k p JB1 PERM.
+        erewrite <- external_call_stack_blocks. 2: eauto.
+        destruct (j b) eqn:A. destruct p0.
+        exploit INCR. eauto. eauto. intro JB2. rewrite JB1 in JB2; inv JB2.
+        eapply NIB; eauto.
+        eapply Mem.perm_max in PERM.
+        eapply external_call_max_perm in PERM.
+        2: eauto.
+        eauto.
+        eapply Mem.valid_block_inject_1; eauto.
+        exploit SEP. eauto. eauto. intuition congruence.
+      + erewrite <- external_call_stack_blocks. 2: eauto.
+        eapply inject_stack_incr; eauto.
+      + 
+        red.
+        unfold Mem.get_frame_info.
+        erewrite <- external_call_stack_blocks. 2: eauto.
+        intros.
 
+        exploit inj_incr_sep_same. eauto. eauto. apply H7. auto.
+        exploit inj_incr_sep_same. eauto. eauto. apply H9. auto.
+        intros.
+        eapply IP; eauto.
+        eapply Mem.perm_max in H10.
+        eapply external_call_max_perm; eauto.
+        eapply Mem.valid_block_inject_1 in H11; eauto.
+      + erewrite <- external_call_stack_blocks. 2: eauto.
+        eapply perm_stack_inv. eauto.
+        apply Mem.in_frames_valid.
+        eapply external_call_perm_frames; eauto.
+      + erewrite <- external_call_stack_blocks. 2: eauto.
+        eapply load_rsp_inv'. eauto.
+        eapply Mem.unchanged_on_implies.
+        eapply external_call_unchanged_on. eauto.
+        unfold Mem.strong_non_private_stack_access.
+        unfold Mem.get_frame_info.
+        intros b ofs0 ; generalize (Mem.stack_adt m). clear.
+        induction l; simpl; intros; eauto.
+
+        destruct a.
+        simpl in *.
+        red in H.
+        simpl in H.
+        destruct o.
+        destruct f.
+        destruct peq. subst.
+        destruct o.
+        eapply in_link_not_in_data; eauto.
+        easy.
+        destr_in H.
+        eapply in_link_not_in_data; eauto.
+        destruct in_dec. easy.
+        destr_in H.
+        eapply in_link_not_in_data; eauto.
+        destr_in H.
+        eapply in_link_not_in_data; eauto.
+      + intros.
+        eapply INCR; eauto.
+      + intros.
+        eapply INCR; eauto.
+      + destruct GLOBSYMB_INJ.
+        split. intros.
+        eapply INCR; eauto.
+        intros.
+        destruct (j b1) eqn:JB1.
+        destruct p.
+        exploit INCR; eauto. rewrite H9; intro X; inv X.
+        eauto.
+        exploit SEP; eauto. intros (NV1 & NV2).
+        simpl; unfold Genv.block_is_volatile.
+        
+        rewrite ! find_var_info_none_ge.
+        auto.
+        unfold Mem.valid_block in NV1. xomega.
+        unfold Mem.valid_block in NV2. xomega.
+      + etransitivity. apply GlobLe. eapply external_call_nextblock; eauto.
+      + etransitivity. apply GlobLeT. eapply external_call_nextblock; eauto.
+      
+    -
+
+      edestruct (extcall_arguments_inject) as (vargs' & Hargs & Hargsinj).
+      eauto.
+      eauto. eauto. 
+      edestruct (external_call_mem_inject_gen ef ge ge)
+        as (j' & vres' & m2' & EC & RESinj & MemInj & Unch1 & Unch2 & INCR & SEP).
+      apply meminj_preserves_globals'_symbols_inject. eauto.
+      eauto.
+      eauto.
+      eauto. 
+      generalize (RINJ PC); rewrite H. inversion 1; subst.
+      assert (j b = Some (b,0)) as JB.
+      {
+        eapply GLOBFUN_INJ. eauto.
+      }
+      rewrite JB in H8; inv H8. 
+      
+      do 3 eexists; split.
+      eapply exec_step_external.
+      eauto.
+      eauto.
+      eauto.
+      generalize (RINJ RSP). destruct (rs RSP); simpl in *; inversion 1; subst; try congruence.
+      destruct Tptr; try easy.
+      destruct Tptr; try easy.
+      destruct Tptr; try easy.
+      destruct Tptr; try easy.
+      generalize (RINJ RA). destruct (rs RA); simpl in *; inversion 1; subst; try congruence.
+      destruct Tptr; try easy.
+      destruct Tptr; try easy.
+      destruct Tptr; try easy.
+      destruct Tptr; try easy.
+      generalize (RINJ RSP). destruct (rs RSP); simpl in *; inversion 1; subst; try congruence.
+      generalize (RINJ RA). destruct (rs RA); simpl in *; inversion 1; subst; try congruence.
+      eauto.
+      reflexivity.
+      econstructor.
+      + eauto.
+      +
+
+        Lemma set_pair_no_rsp:
+          forall p res rs,
+            no_rsp_pair p ->
+            set_pair p res rs RSP = rs RSP.
+        Proof.
+          destruct p; simpl; intros; rewrite ! Pregmap.gso; intuition. 
+        Qed.
+        repeat rewrite Pregmap.gso by (congruence). 
+        rewrite set_pair_no_rsp.
+        rewrite Asmgenproof0.undef_regs_other.
+        rewrite Asmgenproof0.undef_regs_other.
+        eauto.
+        intros; intro; subst. rewrite in_map_iff in H5.
+        destruct H5 as (x & EQ & IN).
+        apply preg_of_not_rsp in EQ. congruence.
+        intros; intro; subst. clear - H5; simpl in *; intuition congruence.
+        auto.
+      + intros; apply val_inject_set.
+        intros; apply val_inject_set.
+
+        Lemma val_inject_set_pair:
+          forall j p res1 res2 rs1 rs2,
+            (forall r, Val.inject j (rs1 r) (rs2 r)) ->
+            Val.inject j res1 res2 ->
+            forall r,
+              Val.inject j (set_pair p res1 rs1 r) (set_pair p res2 rs2 r).
+        Proof.
+          destruct p; simpl; intros; eauto.
+          apply val_inject_set; auto.
+          repeat (intros; apply val_inject_set; auto).
+          apply Val.hiword_inject; auto.
+          apply Val.loword_inject; auto.
+        Qed.
+        intros; apply val_inject_set_pair; auto.
+        apply val_inject_undef_regs; auto.
+        apply val_inject_undef_regs; auto.
+        intros; eapply val_inject_incr; eauto.
+        intros; eapply val_inject_incr; eauto.
+        auto.
+      + eapply external_call_valid_block; eauto.
+      + red. repeat rewrite Pregmap.gso by (congruence). 
+        rewrite set_pair_no_rsp.
+        rewrite Asmgenproof0.undef_regs_other.
+        rewrite Asmgenproof0.undef_regs_other.
+        erewrite <- external_call_stack_blocks. eauto. eauto.
+        intros; intro; subst. rewrite in_map_iff in H5.
+        destruct H5 as (x & EQ & IN).
+        apply preg_of_not_rsp in EQ. congruence.
+        intros; intro; subst. clear - H5; simpl in *; intuition congruence.
+        auto.
+      + erewrite <- external_call_stack_blocks. 2: eauto.
+        repeat rewrite Pregmap.gso by (congruence). 
+        rewrite set_pair_no_rsp.
+        rewrite Asmgenproof0.undef_regs_other.
+        rewrite Asmgenproof0.undef_regs_other.
+        eauto.
+        intros; intro; subst. rewrite in_map_iff in H5.
+        destruct H5 as (x & EQ & IN).
+        apply preg_of_not_rsp in EQ. congruence.
+        intros; intro; subst. clear - H5; simpl in *; intuition congruence.
+        auto. 
+      + red.
+        repeat rewrite Pregmap.gso by (congruence). 
+        rewrite set_pair_no_rsp.
+        rewrite Asmgenproof0.undef_regs_other.
+        rewrite Asmgenproof0.undef_regs_other.
+        eauto.
+        intros; intro; subst. rewrite in_map_iff in H5.
+        destruct H5 as (x & EQ & IN).
+        apply preg_of_not_rsp in EQ. congruence.
+        intros; intro; subst. clear - H5; simpl in *; intuition congruence.
+        auto.
+      + red.
+        intros.
+        eapply Mem.perm_max in H5.
+        eapply external_call_max_perm in H5.
+        2: eauto.
+        eauto. eauto.
+      + red.
+        intros.
+        eapply external_call_perm_bstack. eauto.
+        eauto. 
+      + red.
+        erewrite <- external_call_stack_blocks. 2: eauto.
+        eauto.
+      + repeat rewrite Pregmap.gso by (congruence). 
+        rewrite set_pair_no_rsp.
+        rewrite Asmgenproof0.undef_regs_other.
+        rewrite Asmgenproof0.undef_regs_other.
+        eauto.
+        intros; intro; subst. rewrite in_map_iff in H5.
+        destruct H5 as (x & EQ & IN).
+        apply preg_of_not_rsp in EQ. congruence.
+        intros; intro; subst. clear - H5; simpl in *; intuition congruence.
+        auto. 
+      + red. intros b delta o k p JB1 PERM.
+        erewrite <- external_call_stack_blocks. 2: eauto.
+        destruct (j b) eqn:A. destruct p0.
+        exploit INCR. eauto. eauto. intro JB2. rewrite JB1 in JB2; inv JB2.
+        eapply NIB; eauto.
+        eapply Mem.perm_max in PERM.
+        eapply external_call_max_perm in PERM.
+        2: eauto.
+        eauto.
+        eapply Mem.valid_block_inject_1; eauto.
+        exploit SEP. eauto. eauto. intuition congruence.
+      + erewrite <- external_call_stack_blocks. 2: eauto.
+        eapply inject_stack_incr; eauto.
+      + 
+        red.
+        unfold Mem.get_frame_info.
+        erewrite <- external_call_stack_blocks. 2: eauto.
+        intros.
+
+        exploit inj_incr_sep_same. eauto. eauto. apply H6. auto.
+        exploit inj_incr_sep_same. eauto. eauto. apply H8. auto.
+        intros.
+        eapply IP; eauto.
+        eapply Mem.perm_max in H9.
+        eapply external_call_max_perm; eauto.
+        eapply Mem.valid_block_inject_1 in H10; eauto.
+      + erewrite <- external_call_stack_blocks. 2: eauto.
+        eapply perm_stack_inv. eauto.
+        apply Mem.in_frames_valid.
+        eapply external_call_perm_frames; eauto.
+      + erewrite <- external_call_stack_blocks. 2: eauto.
+        eapply load_rsp_inv'. eauto.
+        eapply Mem.unchanged_on_implies.
+        eapply external_call_unchanged_on. eauto.
+        unfold Mem.strong_non_private_stack_access.
+        unfold Mem.get_frame_info.
+        intros b ofs0 ; generalize (Mem.stack_adt m). clear.
+        induction l; simpl; intros; eauto.
+
+        destruct a.
+        simpl in *.
+        red in H.
+        simpl in H.
+        destruct o.
+        destruct f.
+        destruct peq. subst.
+        destruct o.
+        eapply in_link_not_in_data; eauto.
+        easy.
+        destr_in H.
+        eapply in_link_not_in_data; eauto.
+        destruct in_dec. easy.
+        destr_in H.
+        eapply in_link_not_in_data; eauto.
+        destr_in H.
+        eapply in_link_not_in_data; eauto.
+      + intros.
+        eapply INCR; eauto.
+      + intros.
+        eapply INCR; eauto.
+      + destruct GLOBSYMB_INJ.
+        split. intros.
+        eapply INCR; eauto.
+        intros.
+        destruct (j b1) eqn:JB1.
+        destruct p.
+        exploit INCR; eauto. rewrite H8; intro X; inv X.
+        eauto.
+        exploit SEP; eauto. intros (NV1 & NV2).
+        simpl; unfold Genv.block_is_volatile.
+        
+        rewrite ! find_var_info_none_ge.
+        auto.
+        unfold Mem.valid_block in NV1. xomega.
+        unfold Mem.valid_block in NV2.
+        xomega. 
+      + etransitivity. apply GlobLe. eapply external_call_nextblock; eauto.
+      + etransitivity. apply GlobLeT. eapply external_call_nextblock; eauto.
   Qed.
+
+End PRESERVATION.
+
+  Hypothesis repr_stack_limit:
+    0 <= Memimpl.Mem.stack_limit <= Ptrofs.max_unsigned.
+
+
+  Lemma match_initial_states s:
+    Asm.initial_state prog s ->
+    exists s' j ostack, match_states Vnullptr j ostack s s' /\
+                        mono_initial_state prog s'.
+  Proof.
+    inversion 1. subst.
+    destruct (Mem.alloc m0 0 Memimpl.Mem.stack_limit) as [m1 bstack0] eqn:ALLOC.
+    assert (bstack = bstack0).
+    {
+      unfold bstack.
+      unfold ge.
+      exploit Mem.alloc_result; eauto.
+      erewrite <- Genv.init_mem_genv_next; eauto.
+    }
+    subst.
+    assert (ge = ge0).
+    {
+      unfold ge, ge0. auto.
+    }
+    subst ge0. clear H1.
+    assert (bstack = Mem.nextblock m0) as stackeq.
+    {
+      exploit Mem.alloc_result; eauto.
+    }
+    do 2 eexists; exists (Ptrofs.unsigned Ptrofs.zero); split.
+    2: econstructor; eauto.
+    exploit Genv.initmem_inject; eauto.
+    intro FLATINJ.
+    exploit Mem.alloc_right_inject. apply FLATINJ.
+    eauto. intro STACKINJ.
+    econstructor; eauto.
+    - unfold rs0.
+      rewrite Pregmap.gss. inversion 1.
+    - unfold rs0.
+      intros; apply val_inject_set; auto.
+      intros; apply val_inject_set; auto.
+      intros; apply val_inject_set; auto.
+      + unfold Genv.symbol_address. destr; auto.
+        econstructor. unfold Mem.flat_inj. rewrite pred_dec_true. eauto.
+        erewrite <- Genv.init_mem_genv_next.
+        eapply Genv.genv_symb_range; eauto. eauto. 
+        reflexivity.
+      + constructor.
+      + constructor.
+    - red.         
+      rewrite stackeq. exploit Mem.nextblock_alloc; eauto. intro A; rewrite A; xomega.
+    - red.
+      unfold rs0.
+      rewrite Pregmap.gss. inversion 1.
+    - erewrite Genv.init_mem_stack_adt; eauto.
+    - red. 
+      unfold rs0.
+      rewrite Pregmap.gss. inversion 1.
+    - red. intros.
+      eapply Mem.perm_alloc_3 in H1. 2: eauto.
+      split. omega. eapply Z.lt_le_trans. apply H1. apply repr_stack_limit.
+    - red; intros.
+      eapply Mem.perm_implies. eapply Mem.perm_alloc_2; eauto. constructor.
+    - red. erewrite Mem.alloc_stack_blocks; eauto.
+      erewrite Genv.init_mem_stack_adt; eauto.
+    - unfold rs0.
+      rewrite Pregmap.gss. inversion 1.
+    - red.
+      unfold Mem.flat_inj.
+      intros b delta o k p INJ PERM.
+      destr_in INJ. inv INJ.
+      exploit Mem.alloc_result; eauto. intro; subst. exfalso; clear - H1 p0. rewrite H1 in p0. xomega.
+    -
+      erewrite Genv.init_mem_stack_adt; eauto.
+      constructor.
+    - red. unfold Mem.get_frame_info.
+      erewrite Genv.init_mem_stack_adt; eauto.
+      simpl. congruence.
+    - erewrite Genv.init_mem_stack_adt; eauto. constructor.
+    - erewrite Genv.init_mem_stack_adt; eauto. constructor.
+    - intros. unfold Mem.flat_inj. rewrite pred_dec_true; auto.
+      eapply Genv.find_funct_ptr_not_fresh; eauto.
+    - intros. unfold Mem.flat_inj. rewrite pred_dec_true; auto.
+      eapply Genv.find_def_not_fresh; eauto.
+    - split.
+      simpl; intros; unfold Mem.flat_inj.
+      rewrite pred_dec_true; auto.
+      eapply Genv.find_symbol_not_fresh; eauto.
+      simpl; intros b1 b2 delta; unfold Mem.flat_inj.
+      intro A; destr_in A.
+    - erewrite <- Genv.init_mem_genv_next; eauto. unfold ge; apply Ple_refl.
+    - erewrite Mem.nextblock_alloc.  erewrite <- Genv.init_mem_genv_next; eauto. unfold ge; xomega.
+      eauto.
+  Qed.
+
+  Lemma transf_final_states:
+    forall isp j o st1 st2 r,
+      match_states isp j o st1 st2 -> Asm.final_state st1 r -> final_state st2 r.
+  Proof.
+    inversion 1; subst.
+    inversion 1; subst.
+    econstructor.
+    generalize (RINJ PC). rewrite H3. unfold Vnullptr. destruct ptr64; inversion 1; auto.
+    generalize (RINJ RAX). rewrite H5. unfold Vnullptr. destruct ptr64; inversion 1; auto.
+  Qed.
+
+End WITHMEMORYMODEL.
+
+
+Print Assumptions step_simulation.
